ADD: new archticture

Exec.fst
@@ -28,27 +28,6 @@ let makeFrame virM code localplus global_names local_names =
   let newVM: vm = {virM with callStack = frame::(virM.callStack)} in
   (newVM, frame)
 
-(*
-  Req:
-  Ens:
-*)
-let call_function i globals dataStack =
-  let args, newDataStack = List.splitAt i dataStack in
-  let localplus = List.Tot.Base.rev args in
-  let code, newDataStack = List.splitAt 1 newDataStack in
-  let empty_map = Map.const_on (Set.empty) NONE in
-  match List.hd code with
-  | CODEOBJECT co ->  
-    let newFrame: frameObj = {
-      dataStack = []; 
-      blockStack = [];
-      fCode = co;
-      f_localplus = localplus;
-      pc = 0;
-      f_globals = globals;
-      f_locals = empty_map
-    } in (FRAMEOBJECT newFrame)::dataStack
-  | _ -> All.failwith "CALL_FUNCTION: didn't call a function object"
   
 (*
    Req: length(datastack) >= 1
@@ -108,234 +87,23 @@ let dup_top_two datastack =
 
 
 (*
-   Req: length(datastack) >= 1
-   Ens: 
-     - if tos = INT(i) then res = INT(+i)
-     - if tos = BOOL(b) then res = INT(if b then 1 else 0)
-     - else ERR
-*)
-let unary_positive datastack = 
-  let tos = List.hd datastack in
-  let newDataStack = List.tail datastack in
-  match tos with
-  | INT i -> INT(i)::newDataStack
-  | BOOL b -> INT(if b then 1 else 0)::newDataStack
-  | _ -> ERR("Error: bad operand type for unary +")::newDataStack
-
-(*
-   Req: length(datastack) >= 1
-   Ens: 
-     - if tos = INT(i) then res = INT(-i)
-     - if tos = BOOL(b) then res = INT(if b then -1 else 0)
-     - else ERR
-*)
-let unary_negative datastack = 
-  let tos = List.hd datastack in
-  let newDataStack = List.tail datastack in
-  match tos with
-  | INT i -> INT(-i)::newDataStack
-  | BOOL b -> INT(if b then -1 else 0)::newDataStack
-  | _ -> ERR("Error: bad operand type for unary -")::newDataStack
-
-(*
-   Req: length(datastack) >= 1
-   Ens:
-     - if tos = INT(i)
-     - if tos = STRING(s)
-     - if tos = BOOL(b)
-     - if tos = NONE 
-*)
-let unary_not datastack = 
-  let tos = List.hd datastack in
-  let newDataStack = List.tail datastack in
-  match tos with
-  | INT i -> BOOL(if i=0 then true else false)::newDataStack
-  | STRING s -> BOOL(if s="" then true else false)::newDataStack
-  | BOOL b -> BOOL(if b then false else true)::newDataStack
-  | LIST l -> BOOL(match l with [] -> true | _ -> false)::newDataStack
-  | TUPLE t -> BOOL(match t with [] -> true | _ -> false)::newDataStack
-  | NONE -> BOOL(true)::newDataStack
-  | _ -> ERR("Error: bad operand type for unary -")::newDataStack
-
-(*
-  Req: length(datastack) >= 2
-  Ens:
-    - if tos and tos1 are int(i1), int(i2) or bool(b1), bool(b2):
-      - res = i1*i2, or res = b1 * b2
-    - if tos and tos1 are List(l), int(i) or List(l), bool(b):
-      - res = a list of the items of l repeated i (or b) times
-      - if i <= 0 then res = []
-    - else: res = ERR
-*)
-let binary_multiply (dataStack: list pyObj) = 
-  let tos = List.hd dataStack in
-  let tos1 = List.nth dataStack 1 in
-  let (_, newDataStack) = List.splitAt 2 dataStack in 
-  match (tos, tos1) with
-  | INT(i1), INT(i2) -> INT(op_Multiply i2 i1)::newDataStack
-  | BOOL(b1), BOOL(b2) -> INT(if b1&&b2 then 1 else 0)::newDataStack
-  | BOOL(b), INT(i) -> INT(if b then i else  0)::newDataStack
-  | INT(i), BOOL(b) -> INT(if b then i else 0)::newDataStack
-  | LIST(l), INT(i) ->
-    if 0 >= i 
-    then LIST([])::newDataStack
-    else
-      let l' = List.fold_left (fun x y -> List.append x y) ([]) (tabulate (fun x -> l) i) in
-      LIST(l')::newDataStack
-  | INT(i), LIST(l) -> 
-    if 0 >= i 
-    then LIST([])::newDataStack
-    else
-      let l' = List.fold_left (fun x y -> List.append x y) ([]) (tabulate (fun x -> l) i) in
-      LIST(l')::newDataStack
-  | LIST(l), BOOL(b) -> if b then LIST(l)::newDataStack else LIST([])::newDataStack
-  | BOOL(b), LIST(l) -> if b then LIST(l)::newDataStack else LIST([])::newDataStack
-  | TUPLE(t), INT(i) ->
-    if 0 >= i 
-    then TUPLE([])::newDataStack
-    else
-      let t' = List.fold_left (fun x y -> List.append x y) ([]) (tabulate (fun x -> t) i) in
-      TUPLE(t')::newDataStack
-  | TUPLE(t), BOOL(b) -> if b then TUPLE(t)::newDataStack else TUPLE([])::newDataStack  
-  | _, _ -> ERR("Error: unsupported operand type(s) for *")::newDataStack
-
-(*
-  Req: length(datastack) >= 2
-  ENS:
-    - if tos and tos1 are int(a), int(b) or bool(b1), bool(b2)
-      - res = b // a (or b2 // b1) if a <> 0 (or b1 <> 0)
-      - res = ERR if a == 0 (or b1 == 0)
-*)
-let binary_floor_divide (dataStack: list pyObj) = 
-  let tos = List.hd dataStack in
-  let tos1 = List.nth dataStack 1 in
-  let (_, newDataStack) = List.splitAt 2 dataStack in 
-  match (tos, tos1) with
-  | INT(a), INT(b) -> (if a=0 then ERR("Error: division by zero") else INT(b/a))::newDataStack
-  | BOOL(b1), BOOL(b2) -> (if not b1 then ERR("Error: division by zero") else if b2 then INT(1/1) else INT(0/1))::newDataStack
-  | INT(i), BOOL(b2) -> (if i=0 then ERR("Error: division by zero") else if b2 then INT(1/i) else INT(0/i))::newDataStack
-  | BOOL(b1), INT(i) -> (if not b1 then ERR("Error: division by zero") else INT(i/1))::newDataStack
-  | _, _ -> ERR("Error: unsupported operand type(s) for //")::newDataStack
-
-(*
-  Req: length(datastack) >= 2
-  ENS:
-    - if tos and tos1 are int(a), int(b) or bool(b1), bool(b2)
-      - res = b % a (or b2 % b1) if a <> 0 (or b1 <> 0)
-      - res = ERR if a == 0 (or b1 == 0)
-*)
-let binary_modulo (dataStack: list pyObj) = 
-  let tos = List.hd dataStack in
-  let tos1 = List.nth dataStack 1 in
-  let (_, newDataStack) = List.splitAt 2 dataStack in 
-  match (tos, tos1) with
-  | INT(a), INT(b) -> (if a=0 then ERR("Error: modulo by zero") else INT(b%a))::newDataStack
-  | BOOL(b1), BOOL(b2) -> (if not b1 then ERR("Error: modulo by zero") else if b2 then INT(1%1) else INT(0%1))::newDataStack
-  | INT(i), BOOL(b2) -> (if i=0 then ERR("Error: modulo by zero") else if b2 then INT(1%i) else INT(0%i))::newDataStack
-  | BOOL(b1), INT(i) -> (if not b1 then ERR("Error: modulo by zero") else INT(i%1))::newDataStack
-  | _, _ -> ERR("Error: unsupported operand type(s) for %")::newDataStack
-
-(*
   Req: length(datastack) >= 2
   Ens: 
-    - if tos and tos1 are INT(i1)/BOOL(b1) and INT(i2)/BOOL(b2):
-      - res = INT(i1 + i2) (or b1,b2)
-    - if tos and tos1 are STRING(s1) and STRING(s2):
-      - res = STRING(s1 ^ s2)
-    - if tos and tos1 are LIST(l1) and LIST(l2):
-      - res = LIST(l1 @ l2)
-    - if tos and tos1 are TUPLE(t1) and TUPLE(t2):
-      - res = TUPLE(t1 @ t2)
-    - else:
-      - res = ERR
 *)
 let binary_add (dataStack: list pyObj) = 
   let tos = List.hd dataStack in
   let tos1 = List.nth dataStack 1 in
   let (_, newDataStack) = List.splitAt 2 dataStack in 
   match (tos, tos1) with
-  | TYP(obj1), TYP(obj2) -> match obj1.methods."+" with
-                           | BINFUN f -> match f (obj1.value, obj2.value) with
-                                        | bltin -> builtinsToPyObj bltin
-                                        | NONE -> ERR ("Cannot add objects.")::newDataStack
-                           | _ -> (* No add method *)
-  | INT(a), INT(b) -> INT(b + a)::newDataStack
-  | BOOL(b1), BOOL(b2) -> INT(if b1&&b2 then 2 else if b1||b2 then 1 else 0)::newDataStack
-  | BOOL(b1), INT(i) -> INT(if b1 then 1+i else  0+i)::newDataStack
-  | INT(i), BOOL(b2) -> INT(if b2 then 1+i else 0+i)::newDataStack
-  | STRING(s1), STRING(s2) -> STRING(s2 ^  s1)::newDataStack
-  | LIST(l1), LIST(l2) -> LIST(List.append l1 l2)::newDataStack
-  | TUPLE(t1), TUPLE(t2) -> LIST(List.append t1 t2)::newDataStack
-  | _, _ -> ERR("Error: unsupported operand type(s) for +")::newDataStack
- 
-(*
-  Req: length(datastack) >= 2
-  Ens:
-    - if tos and tos1 are INT(i1) and INT(i2) or(BOOL(b1) and BOOL(b2)):
-      - res = INT(i2 - i1), or(b1, b2)
-    - else:
-      - res = ERR
-*)
-let binary_subtract (dataStack: list pyObj) = 
-  let tos = List.hd dataStack in
-  let tos1 = List.nth dataStack 1 in
-  let (_, newDataStack) = List.splitAt 2 dataStack in 
-  match (tos, tos1) with
-  | INT(a), INT(b) -> INT(b - a)::newDataStack
-  | BOOL(b1), BOOL(b2) -> INT(if b1&&b2 then 0 else if b1 then -1 else if b2 then 1 else 0)::newDataStack
-  | BOOL(b1), INT(i) -> INT(if b1 then i-1 else  i-0)::newDataStack
-  | INT(i), BOOL(b2) -> INT(if b2 then 1+i else 0+i)::newDataStack
-  | _, _ -> ERR("Error: unsupported operand type(s) for -")::newDataStack
-  
-(*
-  Req: length(datastack) >= 2
-  Ens: TOS = TOS1[TOS]
-*)
-let binary_subscr (dataStack: list pyObj) = 
-  let tos = List.hd dataStack in
-  let tos1 = List.nth dataStack 1 in
-  let (_, newDataStack) = List.splitAt 2 dataStack in 
-  match (tos1, tos) with
-  | STRING(s), INT(i) ->
-    let c = if i >= 0 then (subString_pos s i) else (subString_neg s i) in
-     ( match c with
-      | Some c' -> STRING(c')::newDataStack
-      | None -> ERR("Error: String index out of range")::newDataStack)
-  | STRING(s), BOOL(b) -> 
-    let c = if b then (subString_pos s 1) else (subString_neg s 0) in
-      (match c with
-      | Some c' -> STRING(c')::newDataStack
-      | None -> ERR("Error: String index out of range")::newDataStack)
-  | LIST(l), INT(i) -> 
-    let e = 
-      if i >= 0 then (List.Tot.Base.nth l i)
-      else if (-i > List.length l) then None
-      else (List.Tot.Base.nth l ((List.length l) - i))
-    in
-     ( match e with
-      | Some e' -> e'::newDataStack
-      | None ->  ERR("Error: List index out of range")::newDataStack)
-  | LIST(l), BOOL(b) ->
-    let e = if b then (List.Tot.Base.nth l 1) else (List.Tot.Base.nth l 0) in
-     ( match e with
-      | Some e' -> e'::newDataStack
-      | None -> ERR("Error: List index out of range")::newDataStack)
-  | TUPLE(t), INT(i) ->
-    let e = 
-      if i >= 0 then (List.Tot.Base.nth t i)
-      else if (-i > List.length t) then None
-      else (List.Tot.Base.nth t ((List.length t) - i))
-    in
-     ( match e with
-      | Some e' -> e'::newDataStack
-      | None ->  ERR("Error: Tuple index out of range")::newDataStack)
-  | TUPLE(t), BOOL(b) ->
-    let e = if b then (List.Tot.Base.nth t 1) else (List.Tot.Base.nth t 0) in
-      (match e with
-      | Some e' -> e'::newDataStack
-      | None -> ERR("Error: Tuple index out of range")::newDataStack)
-  | _, _ -> ERR("Error: object is not subscriptable")::newDataStack
-  
+  | TYP(obj1), TYP(obj2) -> 
+    (match (Map.sel (obj1.methods) "+") with
+    | BINFUN f -> 
+      (match f (obj1.value, obj2.value) with
+      | bltin -> (builtinsToPyObj bltin)::newDataStack
+      | NONE -> ERR("Cannot add objects" ^ obj1.name ^ obj2.name)::newDataStack)
+    | err -> err::newDataStack)
+  | _, _ -> ERR("Cannot add non objects")::newDataStack
+
 (*
   Req:
   Ens:
@@ -344,11 +112,9 @@ let store_name i names f_locals dataStack =
   let name = List.nth names i in
   let tos = List.hd dataStack in
   let _, newDataStack = List.splitAt 1 dataStack in 
-  (match name with
-  | STRING s -> 
-    let newLocals = Map.upd f_locals s tos in
-    (newLocals, newDataStack)
-  | _ -> All.failwith "STORE_NAME: co_names[i] is not STRING")
+  let newLocals = Map.upd f_locals name tos in
+  (newLocals, newDataStack)
+  
   
 (*
   Req: (length(consts) > i) && (length(datastack) >= 1)
@@ -365,143 +131,12 @@ let load_const i consts dataStack =
 *)
 let load_name i names f_locals f_globals dataStack =
   let name = List.nth names i in
-  match name with
-  | STRING s ->
-    (match Map.contains f_locals s with
-     | true -> (Map.sel f_locals s)::dataStack 
-     | false ->
-       (match Map.contains f_globals s with
-        | true -> (Map.sel f_locals s)::dataStack
-        | false -> (ERR ("name " ^ s ^ "is not defined"))::dataStack
-       )
-    )
-  | _ -> All.failwith "LOAD_NAME: co_names[i] is not STRING"
- 
-(*
-  Req: (length(datastack) >= i)
-  Ens: res = LIST([dataStack[0]; dataStack[1], ... dataStrack[i-1]])::newDataStack
-*)
-let build_tuple i dataStack =
-  let elems, newDataStack  = List.splitAt i dataStack in
-  let newDataStack = TUPLE(elems)::newDataStack in
-  newDataStack
-
-(*
-  Req: (length(datastack) >= i)
-  Ens: res = TUPLE([dataStack[0]; dataStack[1], ... dataStrack[i-1]])::newDataStack
-*)
-let build_list i dataStack =
-  let elems, newDataStack  = List.splitAt i dataStack in
-  let newDataStack = LIST(elems)::newDataStack in
-  newDataStack
-
-let lt_op tos1 tos with
-  match (tos1, tos) with
-  | INT(i1), INT(i2) -> BOOL(i1 < i2)
-  | BOOL(b1), BOOL(b2) -> BOOL(if b1 then false else b2)
-  | BOOL(b), INT(i) -> BOOL(if b then 1<i else 0<i)
-  | INT(i), BOOL(b) -> BOOL(if b then i<1 else i<0)
-  | _, _ -> ERR("Error: '<' not supported between these instances")
-
-let le_op tos1 tos =
-  match (tos1, tos) with
-  | INT(i1), INT(i2) -> BOOL(i1 <= i2)
-  | BOOL(b1), BOOL(b2) -> BOOL(if b1 then b2 else true)
-  | BOOL(b), INT(i) -> BOOL(if b then 1<=i else 0<=i)
-  | INT(i), BOOL(b) -> BOOL(if b then i<=1 else i<=0)
-  | _, _ -> ERR("Error: '<' not supported between these instances")
-
-let eq_op tos1 tos =
-  match (tos1, tos) with
-  | INT(i1), INT(i2) -> BOOL(i1=i2)
-  | BOOL(b1), BOOL(b2) -> BOOL(b1=b2)
-  | BOOL(b), INT(i) -> BOOL(if b then i=1 else i=0)
-  | INT(i), BOOL(b) -> BOOL(if b then i=1 else i=0)  
-  | NONE, NONE -> BOOL(true)
-  | _, _ -> ERR("Error: '==' not supported between these instances")
-
-let neq_op tos1 tos =
-  match (tos1, tos) with
-  | INT(i1), INT(i2) -> BOOL(i1<>i2)
-  | BOOL(b1), BOOL(b2) -> BOOL(b1<>b2)
-  | BOOL(b), INT(i) -> BOOL(if b then i<>1 else i<>0)
-  | INT(i), BOOL(b) -> BOOL(if b then i<>1 else i<>0)  
-  | _, _ -> ERR("Error: '!=' not supported between these instances")
-
-let gt_op tos1 tos with
-  match (tos1, tos) with
-  | INT(i1), INT(i2) -> BOOL(i1 > i2)
-  | BOOL(b1), BOOL(b2) -> BOOL(if b1 then not b2 else false)
-  | BOOL(b), INT(i) -> BOOL(if b then 1>i else 0>i)
-  | INT(i), BOOL(b) -> BOOL(if b then i>1 else i>0)
-  | _, _ -> ERR("Error: '>' not supported between these instances")
-
-let ge_op tos1 tos =
-  match (tos1, tos) with
-  | INT(i1), INT(i2) -> BOOL(i1 >= i2)
-  | BOOL(b1), BOOL(b2) -> BOOL(if b1 then true else not b2)
-  | BOOL(b), INT(i) -> BOOL(if b then 1>=i else 0>=i)
-  | INT(i), BOOL(b) -> BOOL(if b then i>=1 else i>=0)
-  | _, _ -> ERR("Error: '>=' not supported between these instances")
-
-(*
-*)
-let compare_op i dataStack = 
-  let tos = List.hd dataStack in
-  let tos1 = List.nth dataStack 1 in
-  let (_, newDataStack) = List.splitAt 2 dataStack in
-  match i with
-  | 0 -> (lt_op tos1 tos)::newDataStack
-  | 1 -> (le_op tos1 tos)::newDataStack
-  | 2 -> (eq_op tos1 tos)::newDataStack
-  | 3 -> (neq_op tos1 tos)::newDataStack
-  | 4 -> (gt_op tos1 tos)::newDataStack
-  | 5 -> (ge_op tos1 tos)::newDataStack
-  | _ -> (ERR "ERR: compare_op is not supported yet")::newDataStack
-
-(*
-  Req:
-  Ens:
-*)
-let pop_jump_if_true i pc dataStack =
-  let tos = List.hd dataStack in
-  let newDataStack = List.tail dataStack in
-  match tos with
-  | BOOL b -> if b then (i/2, newDataStack) else (pc, newDataStack)
-  | _ -> (pc, (ERR "ERR: argument is not a Bool")::newDataStack)
-
-(*
-  Req:
-  Ens:
-*)
-let pop_jump_if_false i pc dataStack =
-  let tos = List.hd dataStack in
-  let newDataStack = List.tail dataStack in
-  match tos with
-  | BOOL b -> if b then (pc, newDataStack) else (i/2, newDataStack)
-  | _ -> (pc, (ERR "ERR: argument is not a Bool")::newDataStack)
-
-(*
-  Req:
-  Ens:
-*)
-let jump_if_true_or_pop i pc dataStack =
-  let tos = List.hd dataStack in
-  let newDataStack = List.tail dataStack in
-  match tos with
-  | BOOL b -> if b then (i/2, dataStack) else (pc, newDataStack)
-  | _ -> (pc, (ERR "ERR: argument is not a Bool")::newDataStack)
-
-(*
-  Req:
-  Ens:
-*)
-let jump_if_false_or_pop i pc dataStack =
-  let tos = List.hd dataStack in
-  let newDataStack = List.tail dataStack in
-  match tos with
-  | BOOL b -> if b then (pc, newDataStack) else (i/2, dataStack)
-  | _ -> (pc, (ERR "ERR: argument is not a Bool")::newDataStack)
+  match Map.contains f_locals name with
+   | true -> (Map.sel f_locals name)::dataStack 
+   | false ->
+     (match Map.contains f_globals name with
+      | true -> (Map.sel f_locals name)::dataStack
+      | false -> (ERR ("name: " ^ name ^ "is not defined"))::dataStack)
  
 (*
   Req:
@@ -509,13 +144,9 @@ let jump_if_false_or_pop i pc dataStack =
 *)
 let load_global i names f_globals dataStack =
   let name = List.nth names i in
-  match name with
-  | STRING s ->
-    (match Map.contains f_globals s with
-     | true -> (Map.sel f_globals s)::dataStack 
-     | false -> (ERR ("name " ^ s ^ "is not defined"))::dataStack
-    )
-  | _ -> All.failwith "LOAD_GLOBAL: co_names[i] is not STRING"
+  match Map.contains f_globals name with
+   | true -> (Map.sel f_globals name)::dataStack 
+   | false -> (ERR ("name: " ^ name ^ "is not defined"))::dataStack
 
 (*
   Req: (length(localplus) > i) && (length(datastack) >= 1)
@@ -543,34 +174,6 @@ let store_fast i localplus dataStack =
          (let newLocalPlus = List.append localplus [tos] in
            (newLocalPlus, newDataStack)) 
        | false -> All.failwith "STORE_FAST: storing out of index")
-  
-(*
-  Req:
-  Ens:
-*)
-let make_function flags globs dataStack =
-  let qualname = List.hd dataStack in
-  let codeobj = List.nth dataStack 1 in
-  let (_, newDataStack) = List.splitAt 2 dataStack in 
-  let func = FUNCTION ({
-    func_Code = codeobj;
-    func_globals = globs;
-    func_name = qualname;
-    func_closure =
-      if flags = 8 then
-      (match List.hd newDataStack with
-       | TUPLE(t) -> TUPLE(t)
-       | _ -> ERR "Expected closure tuple, got someting else") else NONE;
-   
-    func_defaults =
-      if flags = 1 then
-      (match  List.hd newDataStack with
-       | TUPLE(t) -> TUPLE(t)
-       | _ -> ERR "Expected a defaults tuple, got someting else") else NONE;
-  }) in
-    (match flags with
-     | 0 -> func::newDataStack
-     | _ -> func::(List.tail newDataStack))
      
 (*
    Req: len(frame.fcode.bytecode) >= 1
@@ -583,9 +186,6 @@ let rec execBytecode frame =
     let CODE(bc) = frame.fCode.co_code in
     match List.nth bc (frame.pc) with
     | RETURN_VALUE -> frame
-    | CALL_FUNCTION i -> 
-      let newDataStack = call_function i (frame.f_globals) frame.dataStack in
-        ({frame with dataStack = newDataStack})
     | NOP -> execBytecode ({frame with pc = frame.pc+1})
     | POP_TOP ->
       let newDataStack = pop_top frame.dataStack in
@@ -605,66 +205,18 @@ let rec execBytecode frame =
     | DUP_TOP_TWO ->
       let newDataStack = dup_top_two frame.dataStack in
         execBytecode ({frame with dataStack = newDataStack; pc = frame.pc+1})
-    | UNARY_POSITIVE ->
-      let newDataStack = unary_positive frame.dataStack in
-        execBytecode ({frame with dataStack = newDataStack; pc = frame.pc+1})
-    | UNARY_NEGATIVE ->
-      let newDataStack = unary_negative frame.dataStack in
-        execBytecode ({frame with dataStack = newDataStack; pc = frame.pc+1})
-    | UNARY_NOT ->
-      let newDataStack = unary_not frame.dataStack in
-        execBytecode ({frame with dataStack = newDataStack; pc = frame.pc+1})
-    | BINARY_MULTIPLY -> 
-      let newDataStack = binary_multiply (frame.dataStack) in
-        execBytecode ({frame with dataStack = newDataStack; pc = frame.pc+1})
-    | BINARY_FLOOR_DIVIDE -> 
-      let newDataStack = binary_floor_divide (frame.dataStack) in
-        execBytecode ({frame with dataStack = newDataStack; pc = frame.pc+1})    
-    | BINARY_MODULO -> 
-      let newDataStack = binary_modulo (frame.dataStack) in
-        execBytecode ({frame with dataStack = newDataStack; pc = frame.pc+1})
     | BINARY_ADD -> 
       let newDataStack = binary_add (frame.dataStack) in
-        execBytecode ({frame with dataStack = newDataStack; pc = frame.pc+1})    
-    | BINARY_SUBTRACT -> 
-      let newDataStack = binary_subtract (frame.dataStack) in
-        execBytecode ({frame with dataStack = newDataStack; pc = frame.pc+1}) 
-    | BINARY_SUBSCR -> 
-      let newDataStack = binary_subtract (frame.dataStack) in
-        execBytecode ({frame with dataStack = newDataStack; pc = frame.pc+1}) 
+        execBytecode ({frame with dataStack = newDataStack; pc = frame.pc+1})
+    | STORE_NAME(i) ->
+      let newLocals, newDataStack = store_name i (frame.fCode.co_names) (frame.f_locals) (frame.dataStack) in
+        execBytecode ({frame with dataStack = newDataStack; pc = frame.pc+1; f_locals = newLocals})
     | LOAD_CONST(i) ->
       let newDataStack = load_const i (frame.fCode.co_consts) (frame.dataStack) in
         execBytecode ({frame with dataStack = newDataStack; pc = frame.pc+1})
     | LOAD_NAME(i) ->
       let newDataStack = load_name i (frame.fCode.co_names) (frame.f_locals) (frame.f_globals) (frame.dataStack) in
         execBytecode ({frame with dataStack = newDataStack; pc = frame.pc+1})
-    | BUILD_TUPLE(i) ->
-      let newDataStack = build_tuple i (frame.dataStack) in
-        execBytecode ({frame with dataStack = newDataStack; pc = frame.pc+1})
-    | STORE_NAME(i) ->
-      let newLocals, newDataStack = store_name i (frame.fCode.co_names) (frame.f_locals) (frame.dataStack) in
-        execBytecode ({frame with dataStack = newDataStack; pc = frame.pc+1; f_locals = newLocals})
-    |  BUILD_LIST(i) ->
-      let newDataStack = build_list i (frame.dataStack) in
-        execBytecode ({frame with dataStack = newDataStack; pc = frame.pc+1})
-    | JUMP_FORWARD(i) -> execBytecode ({frame with pc = frame.pc + (i/2) + 1})
-    | POP_JUMP_IF_TRUE(i) ->
-      let newPc, newDataStack = pop_jump_if_true i (frame.pc) (frame.dataStack) in
-      let newPc = if frame.pc=newPc then newPc+1 else newPc in
-        execBytecode ({frame with dataStack = newDataStack; pc = newPc})
-    | POP_JUMP_IF_FALSE(i) ->
-      let newPc, newDataStack = pop_jump_if_false i (frame.pc) (frame.dataStack) in
-      let newPc = if frame.pc=newPc then newPc+1 else newPc in
-        execBytecode ({frame with dataStack = newDataStack; pc = newPc})
-    | JUMP_IF_TRUE_OR_POP(i) ->
-      let newPc, newDataStack = jump_if_true_or_pop i (frame.pc) (frame.dataStack) in
-      let newPc = if frame.pc=newPc then newPc+1 else newPc in
-        execBytecode ({frame with dataStack = newDataStack; pc = newPc})
-    | JUMP_IF_FALSE_OR_POP(i) ->
-      let newPc, newDataStack = jump_if_false_or_pop i (frame.pc) (frame.dataStack) in
-      let newPc = if frame.pc=newPc then newPc+1 else newPc in
-        execBytecode ({frame with dataStack = newDataStack; pc = newPc})
-    | JUMP_ABSOLUTE(i) -> execBytecode ({frame with pc = i/2})
     | LOAD_GLOBAL(i) ->
       let newDataStack = load_global i (frame.fCode.co_names) (frame.f_globals) (frame.dataStack) in
         execBytecode ({frame with dataStack = newDataStack; pc = frame.pc+1})
@@ -674,10 +226,7 @@ let rec execBytecode frame =
     | STORE_FAST(i) ->
       let newLocalPlus, newDataStack = store_fast i (frame.f_localplus) (frame.dataStack) in
         execBytecode ({frame with dataStack = newDataStack; pc = frame.pc+1; f_localplus = newLocalPlus})
-    | MAKE_FUNCTION(flags) ->
-      let newDataStack = make_function flags (frame.f_globals) (frame.dataStack) in
-        execBytecode ({frame with dataStack = newDataStack; pc = frame.pc+1})
-   | _ -> All.failwith "daa"
+   | _ -> All.failwith "Instruction is not implemented yet"
 
     
 (*
