Exec.fsti
@@ -7,8 +7,6 @@ open Utils
 
 val makeFrame: vm -> codeObj -> list pyObj -> (Map.t string pyObj) -> (Map.t string pyObj) -> (vm * frameObj)
 
-val call_function:  nat -> (Map.t string pyObj) -> list pyObj -> All.ML (list pyObj)
-
 val pop_top: list pyObj -> All.ML (list pyObj)
 
 val rot_two: list pyObj -> All.ML (list pyObj)
@@ -21,51 +19,19 @@ val dup_top: list pyObj -> All.ML (list pyObj)
 
 val dup_top_two: list pyObj -> All.ML (list pyObj)
 
-val unary_positive: list pyObj -> All.ML (list pyObj)
-
-val unary_negative: list pyObj -> All.ML (list pyObj)
-
-val unary_not: list pyObj -> All.ML (list pyObj)
-
-val binary_multiply: list pyObj -> All.ML (list pyObj)
-
-val binary_floor_divide: list pyObj -> All.ML (list pyObj)
-
-val binary_modulo: list pyObj -> All.ML (list pyObj)
-
 val binary_add: list pyObj -> All.ML (list pyObj)
 
-val binary_subtract: list pyObj -> All.ML (list pyObj)
-
-val binary_subscr: list pyObj -> All.ML (list pyObj)
-
-val store_name: nat -> list pyObj -> Map.t string pyObj -> list pyObj -> All.ML (Map.t string pyObj * list pyObj)
+val store_name: nat -> list string -> Map.t string pyObj -> list pyObj -> All.ML (Map.t string pyObj * list pyObj)
 
 val load_const: nat -> list pyObj -> list pyObj -> All.ML (list pyObj)
 
-val load_name: nat -> list pyObj -> Map.t string pyObj -> Map.t string pyObj -> list pyObj-> All.ML (list pyObj)
+val load_name: nat -> list string -> Map.t string pyObj -> Map.t string pyObj -> list pyObj-> All.ML (list pyObj)
 
-val build_tuple: nat -> list pyObj -> All.ML (list pyObj)
-
-val build_list: nat -> list pyObj -> All.ML (list pyObj)
-
-val compare_op: nat -> list pyObj -> All.ML (list pyObj)
-  
-val pop_jump_if_true: nat -> nat -> list pyObj -> All.ML (nat * list pyObj)
-
-val pop_jump_if_false: nat -> nat -> list pyObj -> All.ML (nat * list pyObj)
-
-val jump_if_true_or_pop: nat -> nat -> list pyObj -> All.ML (nat * list pyObj)
-
-val jump_if_false_or_pop: nat -> nat -> list pyObj -> All.ML (nat * list pyObj)
-
-val load_global: nat -> list pyObj -> Map.t string pyObj -> list pyObj-> All.ML (list pyObj)
+val load_global: nat -> list string -> Map.t string pyObj -> list pyObj-> All.ML (list pyObj)
 
 val load_fast: nat -> list pyObj -> list pyObj -> All.ML (list pyObj)
 
 val store_fast: nat -> list pyObj -> list pyObj -> All.ML (list pyObj * list pyObj)
-
-val make_function: nat -> (Map.t string pyObj) ->list pyObj -> All.ML (list pyObj)
 
 val execBytecode: frameObj -> All.ML (frameObj)
 
