Structs.fst
@@ -41,16 +41,10 @@ type opcode =
 noeq type bytecode = 
   | CODE: l: list opcode -> bytecode
 
-(* Block object *)
-noeq type blockObj = {
-  (* currently executed opcode (type is int in cpyhton) *)
-  b_type: opcode;
-  (* The number of items on the value stack of the frame *)
-  b_level: nat;
-  (* The index of the instruction after the block *)
-  b_handler: nat
-}
-  
+(* =============================================================== *)
+(*                Python Types embeddings in F*                    *)
+(* =============================================================== *)
+
 (* 
    - The main purpose of using pyObj is to trick 
      the typing system into accepting the type wihtout
@@ -71,7 +65,8 @@ noeq type builtins =
   | STRING: string -> builtins
   | BOOL: bool -> builtins
   | LIST: list pyObj  -> builtins
-  | TUPLE: list pyObj -> builtins  
+  | TUPLE: list pyObj -> builtins
+  | FUNCTION: functionObj -> builtins
   | NONE
   
 and pyObj = 
@@ -94,8 +89,8 @@ and type0 = {
 and codeObj = {
   co_code: bytecode;
   co_consts: list pyObj; // elem at index 0 must be None
-  co_varnames: list pyObj;
-  co_names: list pyObj; 
+  co_varnames: list string;
+  co_names: list string; 
 }
 
 (* Frame object *)
@@ -111,26 +106,26 @@ and frameObj = {
   (* f_builtins *)
 }
 
-private let emptyMap: Map.t string pyObj  = Map.const_on (Set.empty) (ERR("UNDEFINED"))
+(* Function object *)
+and functionObj = {
+  func_Code: pyObj; (* CODEOBJECT *)
+  func_globals: Map.t string pyObj; (* DICT *)
+  func_name: pyObj; (* STRING *)
+  func_closure: pyObj; (* TUPLE *)
+  func_defaults: pyObj; (* TUPLE *)
+  (* func_annotations: pyObj; *) (* DICT *)
+  (* func_kwdefaults: pyObj *) (* DICT *)
+} 
 
-(* *)
-let createInt (v:int) = 
-  let obj: type0= {
-    name = "int";
-    pid = 0;
-    value = INT(v);
-    fields = emptyMap;
-    methods = Map.upd emptyMap "+" 
-      (BINFUN (fun (a, b) -> match (a, b) with 
-                          | INT(a), INT(b) -> INT(a + b) 
-                          | _ -> NONE))
-  } in
-  TYP(obj)
-
-let builtinsToPyObj (bltin: builtins) = 
-  match bltin with
-  | INT n -> createInt n
-  | _ -> All.failwith "TODO"
+(* Block object *)
+and blockObj = {
+  (* currently executed opcode (type is int in cpyhton) *)
+  b_type: opcode;
+  (* The number of items on the value stack of the frame *)
+  b_level: nat;
+  (* The index of the instruction after the block *)
+  b_handler: nat
+}
 
 (* VM (thread) *)
 noeq type vm = {
@@ -138,114 +133,3 @@ noeq type vm = {
   code: codeObj
 }
 
-let five = createInt 5
-
-let r:builtins =
-  match five with
-  | TYP(c) -> c.value
-  | _ -> NONE
- 
-
-
-
-(* --------------------------------------------------------------------------- *)
-
-
-
-
-// let emptyMap = Map.const_on (Set.empty) NONE
-
-// type int0 = {id="int"; fields = emptyMap; methods=emptyMap}
-
-// let r = {id="int"; fields = emptyMap; methods=emptyMap}
-
-// let u = int0.id
-// let y = r.id
-
-// let int0: pyObj = 
-//   let obj:type0 = {id="int"; fields = emptyMap; methods=emptyMap} in
-//   INT(obj)
-
-
-// (* The types of data allowed in datastack*)
-// noeq type pyObj =
-//   | INT: int -> pyObj
-//   (*| FLOAT: FStar.Real.real -> pyObj*)
-//   | STRING: string -> pyObj
-//   | BOOL: bool -> pyObj
-//   | LIST: list pyObj -> pyObj
-//   | TUPLE: list pyObj -> pyObj
-//   (*| DICT: Map.t pyObj pyObj -> pyObj*)  
-//   | NONE
-//   | ERR: string -> pyObj
-//   | FUNCTION: functionObj -> pyObj 
-//   | CODEOBJECT: codeObj -> pyObj
-//   | FRAMEOBJECT: frameObj -> pyObj
-
-// (* Function Object *)
-// and functionObj = {
-//   func_Code: pyObj; (* CODEOBJECT *)
-//   func_globals: Map.t string pyObj; (* DICT *)
-//   func_name: pyObj; (* STRING *)
-//   func_closure: pyObj; (* TUPLE *)
-//   func_defaults: pyObj; (* TUPLE *)
-//   (* func_annotations: pyObj; *) (* DICT *)
-//   (* func_kwdefaults: pyObj *) (* DICT *)
-//   (*
-//   .
-//   .
-//   . 
-//   *)
-// } 
-
-// (* object code *)
-// and codeObj = {
-//   co_code: bytecode;
-//   co_consts: list pyObj; // elem at index 0 must be None
-//   co_varnames: list pyObj;
-//   co_names: list pyObj; 
-//   (*
-//   .
-//   .
-//   . 
-//   *)
-// }
-
-// (* Frame object *)
-// and frameObj = {
-//   (* Simulates a stack that handles inputs of different types *)
-//   dataStack: list pyObj;
-//   (* Simulates a stack of blocks*)
-//   blockStack: list blockObj;
-//   (* code Object that is gonna run in this frame *)
-//   fCode: codeObj;
-//   (* bytecode program counter *)
-//   pc: nat;
-//   (* for fast_load and fast_store *)
-//   f_localplus: list pyObj;
-//   (* global names *)
-//   f_globals: Map.t string pyObj;
-//   (* local names *)
-//   f_locals: Map.t string pyObj;
-//   (* built-in names *)
-//   (* f_builtins *)
-//   (*
-//   .
-//   .
-//   . 
-//   *)
-// }
-
-
-// (* VM (thread) *)
-// noeq type vm = {
-//   (* Simulates a stack of frames *)
-//   callStack: list frameObj;
-//   (* Input to vm *)
-//   code: codeObj
-//   (*
-//   .
-//   .
-//   . 
-//   *)
-//}
