VM.fst
@@ -5,13 +5,9 @@ let runCode code =
   (* Init the virtual machine *)
   let initVM: vm = {
     callStack = [];
-    functionsEnv = []; 
     code = code
   } in
-  let empty_map = Map.const_on (Set.empty) NONE in
   (* Create global frame to run the byte code instructions in it *)
-  let  virM, globalFrame = makeFrame initVM code [] empty_map empty_map in
+  let  virM, globalFrame = makeFrame initVM code [] emptyMap emptyMap in
   let  finalVM, result = runFrame virM globalFrame in
   result
-  
- 
